pulse/ulib/LowStar.RST.Array.fsti
@@ -23,7 +23,6 @@ module Seq = FStar.Seq
 module P = LowStar.Permissions
 module MG = FStar.ModifiesGen
 
-open LowStar.Resource
 open LowStar.RST
 
 include LowStar.RST.Array.Views
@@ -34,18 +33,18 @@ val index (#a:Type) (b:A.array a) (i:UInt32.t)
     (fun _ -> UInt32.v i < A.vlength b)
     (fun h0 x h1 ->
       UInt32.v i < A.vlength b /\
-      Seq.index (as_seq b h0) (UInt32.v i) == x /\
+      Seq.index (as_rseq b h0) (UInt32.v i) == x /\
       h0 == h1
     )
 
 val upd (#a:Type) (b:A.array a) (i:UInt32.t) (v:a)
   : RST unit (array_resource b)
     (fun _ -> array_resource b)
-    (fun h0 -> UInt32.v i < A.vlength b /\ P.allows_write (get_perm b h0))
+    (fun h0 -> UInt32.v i < A.vlength b /\ P.allows_write (get_rperm b h0))
     (fun h0 _ h1 -> UInt32.v i < A.vlength b /\
-      as_seq b h1 ==
-      Seq.upd (as_seq b h0) (UInt32.v i) v /\
-      get_perm b h1 == get_perm b h0
+      as_rseq b h1 ==
+      Seq.upd (as_rseq b h0) (UInt32.v i) v /\
+      get_rperm b h1 == get_rperm b h0
     )
 
 val alloc (#a:Type) (init:a) (len:UInt32.t)
@@ -55,14 +54,14 @@ val alloc (#a:Type) (init:a) (len:UInt32.t)
     (fun _ -> UInt32.v len > 0)
     (fun _ b h1 ->
       A.freeable b /\
-      as_seq b h1 == Seq.create (UInt32.v len) init /\
-      get_perm b h1 = FStar.Real.one
+      as_rseq b h1 == Seq.create (UInt32.v len) init /\
+      get_rperm b h1 = FStar.Real.one
     )
 
 val free (#a:Type) (b:A.array a)
   : RST unit (array_resource b)
     (fun _ -> empty_resource)
-    (fun h0 -> A.freeable b /\ P.allows_write (get_perm b h0))
+    (fun h0 -> A.freeable b /\ P.allows_write (get_rperm b h0))
     (fun _ _ _ -> True)
 
 val share (#a:Type) (b:A.array a)
@@ -72,10 +71,10 @@ val share (#a:Type) (b:A.array a)
         (fun _ -> A.vlength b > 0)
         (fun h0 b' h1 ->
           A.vlength b' = A.vlength b /\
-          as_seq b h0 == as_seq b h1 /\
-          as_seq b' h1 == as_seq b h1 /\
-          get_perm b h1 == P.half_permission (get_perm b h0) /\
-          get_perm b' h1  == P.half_permission (get_perm b h0) /\
+          as_rseq b h0 == as_rseq b h1 /\
+          as_rseq b' h1 == as_rseq b h1 /\
+          get_rperm b h1 == P.half_permission (get_rperm b h0) /\
+          get_rperm b' h1  == P.half_permission (get_rperm b h0) /\
           summable_permissions b b' h1
         )
 
@@ -85,8 +84,8 @@ val gather (#a:Type) (b b':A.array a)
     (fun h0 -> A.gatherable b b' /\ summable_permissions b b' h0)
     (fun h0 _ h1 ->
       summable_permissions b b' h0 /\
-      as_seq b h0 == as_seq b h1 /\
-      get_perm b h1 == P.sum_permissions (get_perm b h0) (get_perm b' h0)
+      as_rseq b h0 == as_rseq b h1 /\
+      get_rperm b h1 == P.sum_permissions (get_rperm b h0) (get_rperm b' h0)
     )
 
 
@@ -97,18 +96,18 @@ val split (#a: Type) (b: A.array a) (idx: UInt32.t{UInt32.v idx > 0 /\ UInt32.v 
     (fun _ -> True)
     (fun h0 bs h1 ->
       A.is_split_into b (fst bs, snd bs) /\
-      as_seq (fst bs) h1 == Seq.slice (as_seq b h0) 0 (UInt32.v idx) /\
-      as_seq (snd bs) h1 == Seq.slice (as_seq b h0) (UInt32.v idx) (A.vlength b) /\
-      get_perm (fst bs) h1 == get_perm b h0 /\
-      get_perm (snd bs) h1 == get_perm b h0
+      as_rseq (fst bs) h1 == Seq.slice (as_rseq b h0) 0 (UInt32.v idx) /\
+      as_rseq (snd bs) h1 == Seq.slice (as_rseq b h0) (UInt32.v idx) (A.vlength b) /\
+      get_rperm (fst bs) h1 == get_rperm b h0 /\
+      get_rperm (snd bs) h1 == get_rperm b h0
     )
 
 val glue (#a: Type) (b b1 b2: A.array a)
   : RST unit
     (array_resource b1 <*> array_resource b2)
     (fun _ -> array_resource b)
-    (fun h0 -> A.is_split_into b (b1, b2) /\ get_perm b1 h0 == get_perm b2 h0)
+    (fun h0 -> A.is_split_into b (b1, b2) /\ get_rperm b1 h0 == get_rperm b2 h0)
     (fun h0 _ h1 ->
-      as_seq b h1 == Seq.append (as_seq b1 h0) (as_seq b2 h0) /\
-      get_perm b h1 == get_perm b1 h0
+      as_rseq b h1 == Seq.append (as_rseq b1 h0) (as_rseq b2 h0) /\
+      get_rperm b h1 == get_rperm b1 h0
     )
